factoring out common parsing code

src/tls/HSL.Receive.fst
@@ -43,9 +43,6 @@ let create r =
   let inc_st = B.malloc r (G.hide (Seq.empty, F_none)) 1ul in
   { rgn = r; inc_st = inc_st }
 
-let receive_flight13_ee_c_cv_fin _ _ _ _ = admit()
-let receive_flight13_ee_cr_c_cv_fin _ _ _ _ = admit ()
-
 module HSM13 = Parsers.Handshake13
 module HSMType = Parsers.HandshakeType
 module Fin13 = Parsers.Handshake13_m_finished
@@ -55,120 +52,133 @@ assume val parsing_error : TLSError.error
 assume val unexpected_flight_error : TLSError.error
 assume val bytes_remain_error : TLSError.error
 
-
 let parse_hsm13
-  (#a:Type) (#k:LP.parser_kind) (#p:LP.parser k a)
-  (#cl:LP.clens HSM13.handshake13 a)
+  (#a:Type) (#k:LP.parser_kind{k.LP.parser_kind_subkind == Some LP.ParserStrong})
+  (#p:LP.parser k a) (#cl:LP.clens HSM13.handshake13 a)
   (#gacc:LP.gaccessor HSM13.handshake13_parser p cl)
+  (tag:HSMType.handshakeType)
   (acc:LP.accessor gacc)
-  (b:slice)
-  (from:uint_32)
+  (b:slice) (from:uint_32)
   : Stack (TLSError.result (option (G.erased a & uint_32)))
     (requires fun h ->
       LP.live_slice h b /\
-      from <= b.LP.len)
-    (ensures  fun h0 r h1 ->
-      
-  = 
+      from <= b.LP.len /\
+      (forall (m:HSM13.handshake13).
+         (HSM13.tag_of_handshake13 m == tag) <==> cl.LP.clens_cond m))
+    (ensures fun h0 r h1 ->
+      B.modifies B.loc_none h0 h1 /\
+      (let open FStar.Error in
+       match r with
+       | Error _ -> True
+       | Correct None -> True
+       | Correct (Some (a_msg, pos)) ->
+         from <= pos /\
+         LP.valid HSM13.handshake13_parser h1 b from /\
+         LP.content_length HSM13.handshake13_parser h1 b from == v (pos - from) /\
+         (let msg13 = LP.contents HSM13.handshake13_parser h1 b from in
+          HSM13.tag_of_handshake13 msg13 == tag /\
+          cl.LP.clens_get msg13 == G.reveal a_msg
+    )))
+  = let open FStar.Error in
   
-#set-options "--z3rlimit 50"
-let receive_flight13_ee_fin st b from to =
-  let open FStar.Error in
-  let from0 = from in
-  let pos = HSM13.handshake13_validator b from in
+    let pos = HSM13.handshake13_validator b from in
 
-  if pos >= to || pos = LP.validator_error_not_enough_data then begin
-    let inc_st =
+    if pos <= LP.validator_max_length then begin
+      let parsed_tag = HSMType.handshakeType_reader b from in
+      if parsed_tag = tag then
+        let payload_begin = acc b from in
+        let payload =
+          let h = ST.get () in
+          let payload = LP.contents p h b payload_begin in
+          G.hide payload
+        in
+        Correct (Some (payload, pos))
+      else Error unexpected_flight_error
+    end
+  else if pos = LP.validator_error_not_enough_data then Correct None
+  else Error parsing_error
+
+let save_incremental_state
+  (st:hsl_state) (b:slice) (from to:uint_32) (in_progress:in_progress_flt_t)
+  : Stack unit
+    (requires fun h ->
+      B.live h st.inc_st /\
+      B.live h b.LP.base /\
+      B.loc_disjoint (footprint st) (B.loc_buffer b.LP.base) /\
+      from <= to /\ to <= b.LP.len)
+    (ensures fun h0 _ h1 ->
+      B.modifies (footprint st) h0 h1 /\
+      parsed_bytes st h1 ==
+        Seq.slice (B.as_seq h1 b.LP.base) (v from) (v to) /\
+      in_progress_flt st h1 == in_progress)
+  = let inc_st =
       let h = ST.get () in
       let parsed_bytes = LP.bytes_of_slice_from_to h b from to in
-      let in_progress = F13_ee_fin in
       G.hide (parsed_bytes, in_progress)
     in
-    B.upd st.inc_st 0ul inc_st;
+    B.upd st.inc_st 0ul inc_st
+
+let reset_incremental_state (st:hsl_state)
+  : Stack unit
+    (requires fun h -> B.live h st.inc_st)
+    (ensures fun h0 _ h1 ->
+      B.modifies (footprint st) h0 h1 /\
+      parsed_bytes st h1 == Seq.empty /\
+      in_progress_flt st h1 == F_none)
+  =  let inc_st = G.hide (Seq.empty, F_none) in
+     B.upd st.inc_st 0ul inc_st
+
+let receive_flight13_ee_c_cv_fin _ _ _ _ = admit()
+let receive_flight13_ee_cr_c_cv_fin _ _ _ _ = admit ()
+
+let mk_ee_fin
+  (begin_fin:uint_32)
+  (ee_msg:G.erased EE.handshake13_m_encrypted_extensions) 
+  (fin_msg:G.erased Fin13.handshake13_m_finished)
+  : flight13_ee_fin
+  = Mkflight13_ee_fin begin_fin ee_msg fin_msg
+
+let receive_flight13_ee_fin st b from to =
+  let open FStar.Error in
+
+  let r = parse_hsm13
+            HSMType.Encrypted_extensions
+            HSM13.handshake13_accessor_encrypted_extensions
+            b from in
+  match r with
+  | Error _ -> Error parsing_error
+  | Correct None ->
+    save_incremental_state st b from to F13_ee_fin;
     Correct None
-  end
-  else if pos <= LP.validator_max_length then begin
-    let msg_t = HSMType.handshakeType_reader b from in
-    match msg_t with
-    | HSMType.Encrypted_extensions ->
-      let ee_payload_begin = HSM13.handshake13_accessor_encrypted_extensions b from in
-      let ee_payload =
-        let h = ST.get () in
-        let payload = LP.contents EE.handshake13_m_encrypted_extensions_parser h b ee_payload_begin in
-        G.hide payload
-      in
-      let from = pos in
-      let pos = HSM13.handshake13_validator b from in
-
+  | Correct (Some (ee_payload, fin_begin)) ->
+    let r = parse_hsm13 HSMType.Finished HSM13.handshake13_accessor_finished b fin_begin in
+    match r with
+    | Error _ -> Error parsing_error
+    | Correct None ->
+      save_incremental_state st b from to F13_ee_fin;
+      Correct None
+    | Correct (Some (fin_payload, pos)) ->
       if pos <> to then Error bytes_remain_error
-
-      else if pos <= LP.validator_max_length then begin
-        let msg_t = HSMType.handshakeType_reader b from in
-        match msg_t with
-        | HSMType.Finished ->
-          let fin_payload_begin = HSM13.handshake13_accessor_finished b from in
-          let fin_payload =
-            let h = ST.get () in
-            let payload = LP.contents Fin13.handshake13_m_finished_parser h b fin_payload_begin in
-            G.hide payload
-          in
-          let inc_st = G.hide (Seq.empty, F_none) in
-          B.upd st.inc_st 0ul inc_st;
-          Correct (Some ({ begin_fin = from; ee_msg = ee_payload; fin_msg = fin_payload }))
-        | _ -> Error unexpected_flight_error
+      else begin
+        reset_incremental_state st;
+        Correct (Some (mk_ee_fin fin_begin ee_payload fin_payload))
       end
-
-      else if pos = LP.validator_error_not_enough_data then begin
-        let inc_st =
-          let h = ST.get () in
-          let parsed_bytes = LP.bytes_of_slice_from_to h b from0 to in
-          let in_progress = F13_ee_fin in
-          G.hide (parsed_bytes, in_progress)
-        in
-        B.upd st.inc_st 0ul inc_st;
-        Correct None
-      end
- 
-      else Error parsing_error
-    | _ -> Error unexpected_flight_error
-  end
-  else Error parsing_error
 
 let receive_flight13_fin st b from to =
   let open FStar.Error in
-  
-  let pos = HSM13.handshake13_validator b from in
 
-  if pos <> to then Error bytes_remain_error
-
-  else if pos <= LP.validator_max_length then begin
-    let msg_t = HSMType.handshakeType_reader b from in
-    match msg_t with
-    | HSMType.Finished ->
-      let fin_payload_begin = HSM13.handshake13_accessor_finished b from in
-      let fin_payload =
-        let h = ST.get () in
-        let payload = LP.contents Fin13.handshake13_m_finished_parser h b fin_payload_begin in
-        G.hide payload
-      in
-      let inc_st = G.hide (Seq.empty, F_none) in
-      B.upd st.inc_st 0ul inc_st;
-      Correct (Some ({ fin_msg = fin_payload }))
-    | _ -> Error unexpected_flight_error
-  end
-
-  else if pos = LP.validator_error_not_enough_data then begin
-    let inc_st =
-      let h = ST.get () in
-      let parsed_bytes = LP.bytes_of_slice_from_to h b from to in
-      let in_progress = F13_fin in
-      G.hide (parsed_bytes, in_progress)
-    in
-    B.upd st.inc_st 0ul inc_st;
+  let r = parse_hsm13 HSMType.Finished HSM13.handshake13_accessor_finished b from in
+  match r with
+  | Error _ -> Error parsing_error
+  | Correct None ->
+    save_incremental_state st b from to F13_fin;
     Correct None
-  end
- 
-  else Error parsing_error
+  | Correct (Some (fin_payload, pos)) ->
+    if pos <> to then Error bytes_remain_error
+    else begin
+      reset_incremental_state st;
+      Correct (Some ({ fin_msg = fin_payload }))
+    end
 
 let receive_flight13_c_cv_fin _ _ _ _ = admit ()
 let receive_flight13_eoed _ _ _ _ = admit ()
